protocols/PartialOrderReduction.v
@@ -1634,14 +1634,14 @@ Proof.
 
   - unfold buildUniverse in *; simpl in *.
     destruct (u_id ==n uid); subst; clean_map_lookups.
-    specialize (H3 _ _ s H5); split_ex.
+    specialize (H5 _ _ s H7); split_ex.
     split; simpl; eauto using summarize_user_step.
 
     destruct ru, userData, u_d; unfold build_data_step in *; simpl in *.
     eapply step_back_into_other_user with (u_id2 := u_id) in H6; eauto.
     split_ors; clean_map_lookups; eauto.
-    specialize (H3 _ _ s H0); simpl in *; eauto.
-    specialize (H3 _ _ s H6); simpl in *; eauto.
+    specialize (H5 _ _ s H0); simpl in *; eauto.
+    specialize (H5 _ _ s H6); simpl in *; eauto.
 Qed.
 
 Hint Resolve summarize_univ_step : core.
@@ -2124,27 +2124,6 @@ Qed.
 
 Hint Resolve indexedIdealSteps_ideal_steps : core.
 
-
-(* Inductive indexedModelStep {t__hon t__adv : type} (uid : user_id) : *)
-(*     @ModelState t__hon t__adv  *)
-(*   -> @ModelState t__hon t__adv *)
-(*   -> Prop := *)
-(* | RealSilenti : forall ru ru' iu b, *)
-(*     indexedRealStep uid Silent ru ru' *)
-(*     -> indexedModelStep uid (ru, iu, b) (ru', iu, b) *)
-(* | BothLoudi : forall ru ru' iu iu' iu'' ra ia b, *)
-(*     indexedRealStep uid (Action ra) ru ru' *)
-(*     -> (indexedIdealStep uid Silent) ^* iu iu' *)
-(*     -> indexedIdealStep uid (Action ia) iu' iu'' *)
-(*     -> action_matches ru.(all_ciphers) ru.(all_keys) ra ia *)
-(*     -> labels_align (ru, iu, b) *)
-(*     -> indexedModelStep uid (ru, iu, b) (ru', iu'', b) *)
-(* | Misalignmenti : forall ru ru' iu ra b, *)
-(*     indexedRealStep uid (Action ra) ru ru' *)
-(*     -> ~ labels_align (ru, iu, b) *)
-(*     -> indexedModelStep uid (ru, iu, b) (ru', iu, false) *)
-(* . *)
-
 Inductive indexedModelStep {t__hon t__adv : type} (uid : user_id) :
     @ModelState t__hon t__adv 
   -> @ModelState t__hon t__adv
@@ -2159,15 +2138,17 @@ Inductive indexedModelStep {t__hon t__adv : type} (uid : user_id) :
     -> action_matches ru.(all_ciphers) ru.(all_keys) ra ia
     -> labels_align (ru, iu, b)
     -> indexedModelStep uid (ru, iu, b) (ru', iu'', b)
-| MisalignedOtheri : forall ru ru' iu iu' iu'' ra ia b,
+| MisalignedCanStepi : forall ru ru' iu iu' iu'' ra ia b,
     indexedRealStep uid (Action ra) ru ru'
     -> (indexedIdealStep uid Silent) ^* iu iu'
     -> indexedIdealStep uid (Action ia) iu' iu''
     -> ~ labels_align (ru, iu, b)
     -> indexedModelStep uid (ru, iu, b) (ru', iu'', false)
-| MisalignedMei : forall ru ru' iu iu' ra b,
+| MisalignedCantStepi : forall ru ru' iu iu' ra b,
     indexedRealStep uid (Action ra) ru ru'
-    -> misalignment uid (ru, iu, b) ra iu'
+    -> (indexedIdealStep uid Silent) ^* iu iu'
+    -> (forall lbl iu'', indexedIdealStep uid lbl iu' iu'' -> False)
+    -> ~ labels_align (ru, iu, b)
     -> indexedModelStep uid (ru, iu, b) (ru', iu, false)
 .
 
@@ -2187,63 +2168,94 @@ Proof.
 Qed.
 
 Hint Constructors indexedModelStep indexedIdealStep indexedRealStep : core.
+Hint Resolve action_matches_other_user_silent_step_inv : core.
+
+Lemma falsify_step :
+  forall t__hon t__adv ru ru' iu iu' b b',
+    @step t__hon t__adv (ru, iu, b) (ru', iu', b')
+    -> step (ru, iu, false) (ru', iu', false).
+Proof.
+  intros * STEP.
+  invert STEP; [
+    econstructor 1    
+  | econstructor 2
+  | econstructor 3
+  | econstructor 4 ]; eauto.
+Qed.
 
 Lemma falsify_trace :
   forall t__hon t__adv ru ru' iu iu' b b' i,
     @stepsi t__hon t__adv i (ru,iu,b) (ru',iu',b')
-    -> @stepsi t__hon t__adv i (ru,iu,false) (ru',iu',false).
+    -> stepsi i (ru,iu,false) (ru',iu',false).
 Proof.
-Admitted.
+  induct 1; eauto.
+  - econstructor; eauto.
+  - destruct st' as [[ru0' iu0'] b0'].
+    econstructor.
+    eapply falsify_step; eauto.
+    eapply IHstepsi; eauto.
+Qed.
 
 Lemma silent_step_labels_still_misaligned :
   forall t__hon t__adv ru iu b,
     ~ @labels_align t__hon t__adv (ru,iu,b)
     -> forall uid ru' b',
       indexedRealStep uid Silent ru ru'
+      -> syntactically_safe_U ru
+      -> goodness_predicates ru
       -> ~ @labels_align t__hon t__adv (ru',iu,b').
 Proof.
-Admitted.
+  unfold not, labels_align; intros.
+  invert H0.
+  apply H; intros.
+  invert H0.
 
-(* Lemma silent_step_always_commutes : *)
-(*   forall {t1 t2} (p1 : user_cmd t1) (p2 : user_cmd t2) cs *)
-(*         -> forall cs cs1' cs2' (usrs usrs1' usrs2' : honest_users A) (adv adv1' adv2' : user_data B) gks gks1' gks2' *)
-(*             ks1 ks1' qmsgs1 qmsgs1' mycs1 mycs1' cmd1 cmd1' froms1 froms1' sents1 sents1' cur_n1 cur_n1' *)
+  destruct (uid0 ==n uid); subst; clean_map_lookups.
+  pose proof (user_step_label_deterministic _ _ _ _ _ _ _ _ _ H5 H7); discriminate.
+  destruct ru, userData, userData0; unfold build_data_step in *; simpl in *.
+  unfold syntactically_safe_U in H1;
+    specialize (H1 _ _ _ H6 eq_refl); split_ex.
+  generalize H7; intros LSTEP.
+  eapply silent_step_then_labeled_step with (uid1 := uid0) (uid2 := uid) in H7; eauto.
+  split_ex.
 
+  dt x1.
 
-(*   nextAction protocol0 ?cmd__n *)
+  generalize H5; intros STEP.
+  eapply silent_step_nochange_other_user with (u_id2 := uid0) in H5; eauto.
+  clean_map_lookups.
 
-(* subgoal 2 (ID 3946) is: *)
-(*  summarize protocol ?s *)
-(* subgoal 3 (ID 3947) is: *)
-(*  commutes ?cmd__n ?s *)
+  assert (
+      IRS :
+        indexedRealStep uid0 (Action ra)
+                        (buildUniverse usrs adv cs gks uid
+                                       {|
+                                         key_heap := ks;
+                                         protocol := cmd;
+                                         msg_heap := qmsgs;
+                                         c_heap := mycs;
+                                         from_nons := froms;
+                                         sent_nons := sents;
+                                         cur_nonce := cur_n |})
+                        (buildUniverse usrs1 adv1 cs1 gks1 uid0
+                                       {|
+                                         key_heap := ks1;
+                                         protocol := cmd1;
+                                         msg_heap := qmsgs1;
+                                         c_heap := mycs1;
+                                         from_nons := froms1;
+                                         sent_nons := sents1;
+                                         cur_nonce := cur_n1 |})).
+  econstructor; eauto.
+  simpl; clean_map_lookups; eauto.
+  unfold build_data_step, buildUniverse; simpl; eauto.
 
+  unfold goodness_predicates in *; simpl in *; split_ex.
 
-Lemma silent_step_preserves_misalignment :
-  forall t__hon t__adv ru ru' iu iu' b uid ra,
-    @misalignment t__hon t__adv uid (ru,iu,b) ra iu'
-    -> indexedRealStep uid (Action ra) ru ru'
-    -> goodness_predicates ru
-    -> syntactically_safe_U ru
-    -> forall uid' ru'',
-      uid' <> uid
-      -> indexedRealStep uid' Silent ru ru''
-      -> misalignment uid (ru'',iu,b) ra iu'.
-Proof.
-  intros * MIS RS GP SS * NE RS'.
-  invert RS; invert RS'.
-  destruct ru, userData, userData0;
-    unfold build_data_step in *; simpl in *.
-  invert MIS; [ econstructor 1 | econstructor 2]; eauto.
-  simpl in *.
-  unfold not in *; intros.
-  apply H7; clear H7.
-  unfold goodness_predicates in GP; split_ex; simpl in *.
-  unfold syntactically_safe_U in SS.
-  specialize (SS _ _ _ H eq_refl); split_ex.
+  eapply H3 in IRS; eauto; split_ex.
+  (do 3 eexists); repeat simple apply conj; eauto using action_matches_other_user_silent_step_inv.
   
-  eapply action_matches_other_user_silent_step_inv; eauto.
-  
-Admitted.
+Qed.
 
 Lemma translate_trace_commute :
   forall t__hon t__adv i st st' b,
@@ -2267,10 +2279,6 @@ Lemma translate_trace_commute :
         /\ stepsi i st0 st0'
         /\ fst st0' = fst st'
         /\ ( snd st0' = snd st' \/ (snd st0' = false /\ snd st' = true) )
-            (* \/ snd st' = false *)
-            (* \/ ( ~ labels_align st0 /\ stepsi i st0 (fst st',false) ) *)
-            (* ) *)
-            (* \/ exists st'0, step^* st0 st'0 /\ snd st'0 = false ) *)
 .
 Proof.
   induct 1; intros; eauto.
@@ -2635,27 +2643,27 @@ Proof.
         eapply max_elt_non_stepped_user with (uid := uid) (uid' := uid0) in MAX; eauto; split_ex.
       rename x0 into msg_heap'.
 
-      specialize (IHstepsi _ _ H17 _ _ next); simpl in *.
+      specialize (IHstepsi _ _ H19 _ _ next); simpl in *.
 
-      apply NatMap.O.max_elt_MapsTo in H17; rewrite find_mapsto_iff in H17; clean_map_lookups.
+      apply NatMap.O.max_elt_MapsTo in H19; rewrite find_mapsto_iff in H19; clean_map_lookups.
       eapply commutes_noblock with (usrs := users ru) (usrs1' := usrs0) in next; eauto; split_ex.
       
-      eapply IHstepsi in H14; clear IHstepsi; eauto 2.
+      eapply IHstepsi in H16; clear IHstepsi; eauto 2.
 
       2 : {
         intros.
         destruct (uid0 ==n u_id2); subst; clean_map_lookups; eauto.
-        destruct userData2; eapply step_back_into_other_user with (u_id3 := u_id2) in H13; eauto.
+        destruct userData2; eapply step_back_into_other_user with (u_id3 := u_id2) in H15; eauto.
         split_ors; split_ex; eauto.
       }
       split_ex; subst.
 
-      invert H14; clear_labeled_commuting_steps uid.
+      invert H16; clear_labeled_commuting_steps uid.
 
-      eapply commutes_sound with (u_id1 := uid0) (u_id2 := uid) in H22; eauto.
+      eapply commutes_sound with (u_id1 := uid0) (u_id2 := uid) in H24; eauto.
       split_ex; subst.
 
-      unfold build_data_step in H22; destruct ru; simpl in *.
+      unfold build_data_step in H24; destruct ru; simpl in *.
       dt x13; dt x14; destruct x15; simpl in *.
 
       destruct x12 as [[ru1 iu1] b1].
@@ -2666,545 +2674,10 @@ Proof.
       econstructor 4; eauto.
       econstructor; eauto.
       symmetry; trivial.
-      eapply silent_step_preserves_misalignment; eauto.
+      eapply silent_step_labels_still_misaligned with (b := b0) (b' := b0) in H14; eauto.
       eauto.
       eauto.
 Qed.
-
-
-
-(* Lemma translate_trace_commute : *)
-(*   forall t__hon t__adv i st st' b, *)
-(*     @stepsi t__hon t__adv (1 + i) st st' *)
-(*     -> lameAdv b (fst (fst st)).(adversary) *)
-(*     -> syntactically_safe_U (fst (fst st)) *)
-(*     -> goodness_predicates (fst (fst st)) *)
-(*     -> (forall st'', ~ step st' st'') *)
-(*     -> forall summaries, summarize_univ (fst (fst st)) summaries *)
-(*     -> forall uid ud, NatMap.O.max_elt (fst (fst st)).(users) = Some (uid,ud) *)
-(*     -> forall t (cmd__n : user_cmd t), nextAction ud.(protocol) cmd__n *)
-(*     -> (forall u_id2 userData2, *)
-(*           uid <> u_id2 *)
-(*           -> users (fst (fst st)) $? u_id2 = Some userData2 *)
-(*           -> exists s, *)
-(*                 summaries $? u_id2 = Some s *)
-(*               /\ commutes cmd__n s) *)
-(*     -> forall lbl bd, step_user lbl (Some uid) (build_data_step (fst (fst st)) ud) bd *)
-(*     -> exists st0, *)
-(*             (* step_user lbl' (Some uid) (build_data_step (fst (fst st)) ud) bd' *) *)
-(*             indexedModelStep uid st st0 *)
-(*           (* /\ ru = buildUniverse_step bd' uid *) *)
-(*           /\ stepsi i st0 st' *)
-(*           (* /\ stepsi i (ru, iu, v) st' *) *)
-(*           (* /\ stepsi i (ru, snd (fst st), v) st' *) *)
-(*           (* /\ (match lbl' with *) *)
-(*           (*    | Silent    => (exists v, stepsi i (ru, snd (fst st), v) st') *) *)
-(*           (*    | Action ra => *) *)
-(*           (*      ( exists iu' iu'' ia v, *) *)
-(*           (*          (indexedIdealStep uid Silent)^* (snd (fst st)) iu' *) *)
-(*           (*          /\ indexedIdealStep uid (Action ia) iu' iu'' *) *)
-(*           (*          /\ action_matches (fst (fst st)).(all_ciphers) (fst (fst st)).(all_keys) ra ia *) *)
-(*           (*          /\ labels_align st *) *)
-(*           (*          /\ stepsi i (ru, iu'', v) st') *) *)
-(*           (*      \/ (exists iu' v, *) *)
-(*           (*            (~ labels_align st) *) *)
-(*           (*            /\ stepsi i (ru, iu', v) st') *) *)
-(*           (*    end) *) *)
-(* . *)
-(* Proof. *)
-(*   induct 1; intros; eauto. *)
-
-(*   invert H0. *)
-
-(*   - clear IHstepsi. *)
-(*     invert H; simpl in *; *)
-(*       repeat *)
-(*         match goal with *)
-(*         | [ H : step_universe _ _ _ |- _ ] => invert H; dismiss_adv *)
-(*         | [ H : indexedRealStep _ _ _ _ |- _ ] => invert H *)
-(*         | [ H : O.max_elt _ = Some _ |- _ ] => *)
-(*           apply NatMap.O.max_elt_MapsTo in H; rewrite find_mapsto_iff in H *)
-(*         end. *)
-
-(*     + destruct (uid ==n u_id); subst; clean_map_lookups. *)
-
-(*       (* equal *) *)
-(*       eexists; repeat simple apply conj; simpl; eauto 8. *)
-(*       econstructor 1; eauto. *)
-(*       econstructor 1; eauto. *)
-
-(*       (* not equal *)  *)
-(*       assert (LK : users ru $? u_id = Some userData) by assumption. *)
-(*       eapply H8 in LK; eauto; split_ex. *)
-(*       destruct userData, ud; unfold build_data_step in *; simpl in *. *)
-      
-(*       specialize (H5 _ _ x H); split_ex. *)
-(*       dt bd; unfold buildUniverse in H4. *)
-
-(*       destruct lbl. *)
-(*       * (* usrs ru $? uid *) *)
-(*         generalize H6; intros STEP. *)
-(*         eapply silent_step_nochange_other_user in STEP; eauto. *)
-
-(*         eapply commutes_noblock with (usrs := users ru) (usrs1' := usrs) in (*na*) H7; eauto; split_ex. *)
-(*         exfalso; split_ex; eapply H4; eauto. *)
-(*         econstructor; eauto. *)
-
-(*       * eapply labeled_action_never_commutes in H9; eauto; contradiction. *)
-
-(*     + destruct (uid ==n uid0); subst; clean_map_lookups. *)
-
-(*       (* equal *) *)
-(*       eexists; repeat simple apply conj; simpl; eauto 8. *)
-(*       econstructor 2; eauto. *)
-(*       econstructor; eauto. *)
-
-(*       (* not equal *)  *)
-(*       assert (LK : users ru $? uid0 = Some userData) by assumption. *)
-(*       eapply H8 in LK; eauto; split_ex. *)
-(*       destruct userData, ud; unfold build_data_step in *; simpl in *. *)
-      
-(*       specialize (H5 _ _ x H); split_ex. *)
-(*       dt bd; unfold buildUniverse in H4. *)
-
-(*       destruct lbl. *)
-(*       * (* usrs ru $? uid *) *)
-(*         generalize H6; intros STEP. *)
-(*         eapply step_limited_change_other_user in STEP; eauto; split_ex. *)
-
-(*         split_ors; clean_map_lookups; *)
-(*           eapply commutes_noblock with (usrs := users ru) (usrs1' := usrs) in (*na*) H7; eauto; split_ex; *)
-(*             exfalso; split_ex; eapply H4; eauto; *)
-(*               econstructor; eauto. *)
-
-(*       * eapply labeled_action_never_commutes in H9; eauto; contradiction. *)
-
-(*     + destruct (uid ==n uid0); subst; clean_map_lookups. *)
-
-(*       (* equal *) *)
-(*       eexists; repeat simple apply conj; simpl; eauto 8. *)
-(*       econstructor 3; eauto. *)
-(*       econstructor. *)
-
-(*       (* not equal *)  *)
-(*       assert (LK : users ru $? uid0 = Some userData) by assumption. *)
-(*       eapply H8 in LK; eauto; split_ex. *)
-(*       destruct userData, ud; unfold build_data_step in *; simpl in *. *)
-      
-(*       specialize (H5 _ _ x H); split_ex. *)
-(*       dt bd; unfold buildUniverse in H4. *)
-
-(*       destruct lbl. *)
-(*       * (* usrs ru $? uid *) *)
-(*         generalize H6; intros STEP. *)
-(*         eapply step_limited_change_other_user in STEP; eauto; split_ex. *)
-
-(*         split_ors; clean_map_lookups; *)
-(*           eapply commutes_noblock with (usrs := users ru) (usrs1' := usrs) in (*na*) H7; eauto; split_ex; *)
-(*             exfalso; split_ex; eapply H4; eauto; *)
-(*               econstructor; eauto. *)
-
-(*       * eapply labeled_action_never_commutes in H9; eauto; contradiction. *)
-
-(*     + destruct (uid ==n uid0); subst; clean_map_lookups. *)
-
-(*       (* equal *) *)
-(*       eexists; repeat simple apply conj; simpl; eauto 8. *)
-(*       econstructor 4; eauto. *)
-(*       econstructor. *)
-
-(*       (* not equal *)  *)
-(*       assert (LK : users ru $? uid0 = Some userData) by assumption. *)
-(*       eapply H8 in LK; eauto; split_ex. *)
-(*       destruct userData, ud; unfold build_data_step in *; simpl in *. *)
-      
-(*       specialize (H5 _ _ x H); split_ex. *)
-(*       dt bd; unfold buildUniverse in H4. *)
-
-(*       destruct lbl. *)
-(*       * (* usrs ru $? uid *) *)
-(*         generalize H6; intros STEP. *)
-(*         eapply step_limited_change_other_user in STEP; eauto; split_ex. *)
-
-(*         split_ors; clean_map_lookups; *)
-(*           eapply commutes_noblock with (usrs := users ru) (usrs1' := usrs) in (*na*) H7; eauto; split_ex; *)
-(*             exfalso; split_ex; eapply H4; eauto; *)
-(*               econstructor; eauto. *)
-
-(*       * eapply labeled_action_never_commutes in H9; eauto; contradiction. *)
-
-(*   - assert (LAME: lameAdv b (adversary (fst (fst st)))) by assumption. *)
-(*     eapply adversary_remains_lame_step in LAME; eauto. *)
-
-(*     assert (SUMMARIES : summarize_univ (fst (fst st)) summaries) by assumption. *)
-(*     eapply summarize_univ_step in SUMMARIES; eauto. *)
-
-(*     assert (SS : syntactically_safe_U (fst (fst st'))) by eauto using syntactically_safe_U_preservation_step. *)
-(*     assert (UNIVS : goodness_predicates (fst (fst st'))) by (eapply goodness_preservation_step; eauto). *)
-
-(*     specialize (IHstepsi _ _ eq_refl LAME SS UNIVS H4 _ SUMMARIES). *)
-(*     assert (next : nextAction (protocol ud) cmd__n) by assumption. *)
-
-(*     dt bd; destruct ud; simpl in *. *)
-
-(*     invert H; simpl in *; *)
-(*       match goal with *)
-(*       | [ H : step_universe _ _ _ |- _ ] => invert H; dismiss_adv *)
-(*       | [ H : indexedRealStep _ _ _ _ |- _ ] => invert H *)
-(*       end; *)
-(*       match goal with *)
-(*       | [ H : O.max_elt _ = Some _ |- _ ] => *)
-(*         let MAX := fresh "H" *)
-(*         in generalize H; intros MAX; *)
-(*              apply NatMap.O.max_elt_MapsTo in MAX; rewrite find_mapsto_iff in MAX *)
-(*       end; *)
-(*       try rename u_id into uid0. *)
-
-(*     + destruct (uid ==n uid0); subst; clean_map_lookups. *)
-
-(*       eexists; repeat simple apply conj; eauto. *)
-(*       econstructor; eauto. *)
-(*       econstructor; eauto. *)
-      
-
-(*       assert (LK : users ru $? uid0 = Some userData) by assumption. *)
-(*       eapply H8 in LK; eauto; split_ex. *)
-
-(*       destruct userData; unfold buildUniverse, build_data_step in *; simpl in *. *)
-(*       specialize (H5 _ _ x H); split_ex. *)
-
-(*       generalize H6; intros MAX; *)
-(*         eapply max_elt_non_stepped_user with (uid := uid) (uid' := uid0) in MAX; eauto; split_ex. *)
-(*       rename x0 into msg_heap'. *)
-
-(*       specialize (IHstepsi _ _ H16 _ _ next); simpl in *. *)
-
-(*       apply NatMap.O.max_elt_MapsTo in H16; rewrite find_mapsto_iff in H16; clean_map_lookups. *)
-(*       eapply commutes_noblock with (usrs := users ru) (usrs1' := usrs0) in next; eauto; split_ex. *)
-      
-(*       eapply IHstepsi in H13; clear IHstepsi; eauto 2. *)
-
-(*       2 : { *)
-(*         intros. *)
-(*         destruct (uid0 ==n u_id2); subst; clean_map_lookups; eauto. *)
-(*         destruct userData2; eapply step_back_into_other_user with (u_id3 := u_id2) in H12; eauto. *)
-(*         split_ors; split_ex; eauto. *)
-(*       } *)
-(*       split_ex; subst. *)
-
-(*       Ltac clear_labeled_commuting_steps usr_id := *)
-(*         repeat *)
-(*           match goal with *)
-(*           | [ H : indexedRealStep usr_id _ _ _ |- _ ] => invert H *)
-(*           | [ H : step_user (Action _) (Some usr_id) _ _ |- _ ] => *)
-(*             unfold build_data_step in H *)
-(*             ; simpl in * *)
-(*             ; clean_map_lookups *)
-(*             ; eapply labeled_action_never_commutes in H *)
-(*             ; solve [ contradiction || eauto ] *)
-(*           end. *)
-
-(*       invert H13; clear_labeled_commuting_steps uid. *)
-
-(*       eapply commutes_sound with (u_id1 := uid0) (u_id2 := uid) in H19; eauto. *)
-(*       split_ex; subst. *)
-
-(*       unfold build_data_step in H19; destruct ru; simpl in *. *)
-(*       dt x12; dt x13; destruct x14; simpl in *. *)
-(*       (* dt x13; dt x12; destruct x14; simpl in *. *) *)
-(*       eexists; repeat simple apply conj; eauto. *)
-(*       econstructor 1; eauto. *)
-(*       econstructor; eauto. *)
-      
-(*       econstructor 1; eauto. *)
-(*       econstructor 1; eauto. *)
-(*       rewrite H23; trivial. *)
-
-(*     + destruct (uid ==n uid0); subst; clean_map_lookups. *)
-
-(*       (* equal *) *)
-(*       eexists; repeat simple apply conj; eauto. *)
-(*       econstructor 2; eauto. *)
-(*       econstructor; eauto. *)
-
-(*       (* not equal *) *)
-(*       assert (LK : users ru $? uid0 = Some userData) by assumption. *)
-(*       eapply H8 in LK; eauto; split_ex. *)
-
-(*       destruct userData; unfold buildUniverse, build_data_step in *; simpl in *. *)
-(*       specialize (H5 _ _ x H); split_ex. *)
-
-(*       generalize H6; intros MAX; *)
-(*         eapply max_elt_non_stepped_user with (uid := uid) (uid' := uid0) in MAX; eauto; split_ex. *)
-(*       rename x0 into msg_heap'. *)
-
-(*       specialize (IHstepsi _ _ H20 _ _ next); simpl in *. *)
-
-(*       apply NatMap.O.max_elt_MapsTo in H20; rewrite find_mapsto_iff in H20; clean_map_lookups. *)
-(*       eapply commutes_noblock with (usrs := users ru) (usrs1' := usrs0) in next; eauto; split_ex. *)
-      
-(*       eapply IHstepsi in H17; clear IHstepsi; eauto 2. *)
-
-(*       2 : { *)
-(*         intros. *)
-(*         destruct (uid0 ==n u_id2); subst; clean_map_lookups; eauto. *)
-(*         destruct userData2; eapply step_back_into_other_user with (u_id3 := u_id2) in H16; eauto. *)
-(*         split_ors; split_ex; eauto. *)
-(*       } *)
-(*       split_ex; subst. *)
-
-(*       invert H17; clear_labeled_commuting_steps uid. *)
-
-(*       eapply commutes_sound with (u_id1 := uid0) (u_id2 := uid) in H23; eauto. *)
-(*       split_ex; subst. *)
-
-(*       unfold build_data_step in H23; destruct ru; simpl in *. *)
-(*       dt x12; dt x13; destruct x14; simpl in *. *)
-(*       eexists; repeat simple apply conj; eauto. *)
-(*       econstructor 1; eauto. *)
-
-(*       destruct (classic (labels_align (buildUniverse usrs2 adv2 cs2 gks2 uid *)
-(*                 {| *)
-(*                 key_heap := ks2; *)
-(*                 protocol := cmd2; *)
-(*                 msg_heap := qmsgs2; *)
-(*                 c_heap := mycs2; *)
-(*                 from_nons := froms2; *)
-(*                 sent_nons := sents2; *)
-(*                 cur_nonce := cur_n2 |}, iu, b0))). *)
-
-(*       * econstructor; eauto. *)
-(*         econstructor 2; eauto. *)
-(*         all: simpl. *)
-(*         econstructor; eauto. *)
-(*         rewrite H27; trivial. *)
-
-(*         (* Lemma : action matches after silent step other *) *)
-(*         (* H14 : action_matches all_ciphers all_keys ra ia *) *)
-(*         admit. *)
-
-(*       * econstructor. *)
-(*         econstructor 3; eauto. *)
-(*         (* Here there be dragons *) *)
-        
-      
-(*     + destruct (uid ==n u_id); subst; clean_map_lookups. *)
-
-(*       (* equal *) *)
-(*       (do 5 eexists); repeat simple apply conj; eauto. *)
-(*       econstructor; eauto. *)
-
-(*       (* not equal *) *)
-(*       assert (LK : users ru $? u_id = Some userData) by assumption. *)
-(*       eapply H8 in LK; eauto; split_ex. *)
-
-(*       destruct userData; unfold buildUniverse, build_data_step in *; simpl in *. *)
-(*       specialize (H5 _ _ x H); split_ex. *)
-
-(*       generalize H6; intros MAX; *)
-(*         eapply max_elt_non_stepped_user with (uid := uid) (uid' := u_id) in MAX; eauto; split_ex. *)
-(*       rename x0 into msg_heap'. *)
-
-(*       specialize (IHstepsi _ _ H16 _ _ next); simpl in *. *)
-
-(*       apply NatMap.O.max_elt_MapsTo in H16; rewrite find_mapsto_iff in H16; clean_map_lookups. *)
-(*       eapply commutes_noblock with (usrs := users ru) (usrs1' := usrs0) in next; eauto; split_ex. *)
-      
-(*       eapply IHstepsi in H13; clear IHstepsi; eauto. *)
-
-(*       2 : { *)
-(*         intros. *)
-(*         destruct (u_id ==n u_id2); subst; clean_map_lookups; eauto. *)
-(*         destruct userData2; eapply step_back_into_other_user with (u_id3 := u_id2) in H12; eauto. *)
-(*         split_ors; split_ex; eauto. *)
-(*       } *)
-(*       split_ex; subst. *)
-(*       eapply commutes_sound with (u_id1 := u_id) (u_id2 := uid) in H13; eauto. *)
-(*       split_ex; subst. *)
-(*       2-3: unfold build_data_step, buildUniverse_step; simpl; eauto. *)
-
-(*       unfold build_data_step in H13; destruct ru; simpl in *. *)
-
-(*       (do 3 eexists); repeat simple apply conj; eauto. *)
-(*       destruct x11; split_ex; eauto. *)
-(*       eexists; econstructor; eauto. *)
-(*       dt x14; dt x15; destruct x16; simpl in *. *)
-(*       econstructor 1; eauto. *)
-(*       econstructor 1; eauto. *)
-(*       rewrite <- H22; trivial. *)
-
-(*       dt x14; eapply labeled_action_never_commutes in H13; eauto; contradiction. *)
-
-(*     + destruct (uid ==n uid0); subst; clean_map_lookups. *)
-
-(*       (* equal *) *)
-(*       (do 3 eexists); repeat simple apply conj; eauto 10. *)
-(*       simpl. *)
-
-(*       left. *)
-(*       (do 4 eexists); repeat simple apply conj; eauto. *)
-(*       econstructor; eauto. *)
-
-(*       (* not equal *) *)
-(*       assert (LK : users ru $? uid0 = Some userData) by assumption. *)
-(*       eapply H8 in LK; eauto; split_ex. *)
-
-(*       destruct userData; unfold buildUniverse, build_data_step in *; simpl in *. *)
-(*       specialize (H5 _ _ x H); split_ex. *)
-
-(*       generalize H6; intros MAX; *)
-(*         eapply max_elt_non_stepped_user with (uid := uid) (uid' := uid0) in MAX; eauto; split_ex. *)
-(*       rename x0 into msg_heap'. *)
-
-(*       specialize (IHstepsi _ _ H20 _ _ next); simpl in *. *)
-
-(*       apply NatMap.O.max_elt_MapsTo in H20; rewrite find_mapsto_iff in H20; clean_map_lookups. *)
-
-(*       eapply commutes_noblock with (usrs := users ru) (usrs1' := usrs0) in next; eauto; split_ex. *)
-(*       eapply IHstepsi in H17; clear IHstepsi; eauto. *)
-
-(*       2 : { *)
-(*         intros. *)
-(*         destruct (uid0 ==n u_id2); subst; clean_map_lookups; eauto. *)
-(*         destruct userData2; eapply step_back_into_other_user with (u_id3 := u_id2) in H16; eauto. *)
-(*         split_ors; split_ex; eauto. *)
-(*       } *)
-(*       split_ex; subst. *)
-
-(*       generalize H16; intros; eapply commutes_sound with (u_id1 := uid0) (u_id2 := uid) in H16; eauto. *)
-(*       split_ex; subst. *)
-
-(*       2-3: solve [ unfold build_data_step, buildUniverse_step; simpl; eauto ]. *)
-      
-(*       unfold build_data_step in H16; destruct ru; simpl in *. *)
-(*       (do 3 eexists); repeat simple apply conj; eauto. *)
-(*       destruct x11; split_ex; eauto. *)
-(*       * dt x14; dt x15; destruct x16; simpl in *. *)
-
-(*         destruct ( *)
-(*             classic *)
-(*               (labels_align *)
-(*                  (buildUniverse usrs1 adv1 cs1 gks1 uid *)
-(*                                 {| *)
-(*                                   key_heap := ks1; *)
-(*                                   protocol := cmd1; *)
-(*                                   msg_heap := qmsgs1; *)
-(*                                   c_heap := mycs1; *)
-(*                                   from_nons := froms1; *)
-(*                                   sent_nons := sents1; *)
-(*                                   cur_nonce := cur_n1 |}, iu, b0))). *)
-(*         ** eexists. *)
-(*            econstructor; eauto. *)
-(*            econstructor 2; eauto. *)
-(*            econstructor; eauto. *)
-(*            rewrite H27; trivial. *)
-
-(*            unfold syntactically_safe_U in *; split_ex; simpl in *. *)
-(*            generalize H0; intros USR; eapply H2 in USR; split_ex; eauto; simpl in *. *)
-
-(*            unfold goodness_predicates in *; simpl in *; *)
-(*              split_ex; *)
-(*              eapply action_matches_other_user_silent_step; eauto. *)
-
-(*         ** eexists. *)
-(*            econstructor; eauto. *)
-(*            (* econstructor 3; eauto. *) *)
-(*            (* econstructor; eauto. *) *)
-(*            (* rewrite H27; trivial. *) *)
-(*            admit. *)
-
-(*       * exfalso. *)
-(*         dt x14; unfold build_data_step in H16; eapply labeled_action_never_commutes in H16; eauto; contradiction. *)
-
-(*     (* Third constructor of step *) *)
-(*     + destruct (uid ==n uid0); subst; clean_map_lookups. *)
-
-(*       (* equal *) *)
-(*       (do 3 eexists); repeat simple apply conj; eauto 10. *)
-(*       simpl. *)
-(*       right. *)
-(*       (do 2 eexists); repeat simple apply conj; eauto. *)
-(*       econstructor; eauto. *)
-
-(*       (* not equal *) *)
-(*       assert (LK : users ru $? uid0 = Some userData) by assumption. *)
-(*       eapply H8 in LK; eauto; split_ex. *)
-
-(*       destruct userData; unfold buildUniverse, build_data_step in *; simpl in *. *)
-(*       specialize (H5 _ _ x H); split_ex. *)
-
-(*       generalize H6; intros MAX; *)
-(*         eapply max_elt_non_stepped_user with (uid := uid) (uid' := uid0) in MAX; eauto; split_ex. *)
-(*       rename x0 into msg_heap'. *)
-
-(*       specialize (IHstepsi _ _ H17 _ _ next); simpl in *. *)
-
-(*       apply NatMap.O.max_elt_MapsTo in H17; rewrite find_mapsto_iff in H17; clean_map_lookups. *)
-
-(*       eapply commutes_noblock with (usrs := users ru) (usrs1' := usrs0) in next; eauto; split_ex. *)
-(*       eapply IHstepsi in H14; clear IHstepsi; eauto. *)
-
-(*       2 : { *)
-(*         intros. *)
-(*         destruct (uid0 ==n u_id2); subst; clean_map_lookups; eauto. *)
-(*         destruct userData2; eapply step_back_into_other_user with (u_id3 := u_id2) in H13; eauto. *)
-(*         split_ors; split_ex; eauto. *)
-(*       } *)
-(*       split_ex; subst. *)
-
-(*       generalize H13; intros; eapply commutes_sound with (u_id1 := uid0) (u_id2 := uid) in H13; eauto. *)
-(*       split_ex; subst. *)
-
-(*       2-3: solve [ unfold build_data_step, buildUniverse_step; simpl; eauto ]. *)
-      
-(*       unfold build_data_step in H13; destruct ru; simpl in *. *)
-(*       (do 3 eexists); repeat simple apply conj; eauto. *)
-(*       destruct x11; split_ex; eauto. *)
-
-(*       * dt x14; dt x15; destruct x16; simpl in *. *)
-
-(*         destruct ( *)
-(*             classic *)
-(*               (labels_align *)
-(*                  (buildUniverse usrs1 adv1 cs1 gks1 uid *)
-(*                                 {| *)
-(*                                   key_heap := ks1; *)
-(*                                   protocol := cmd1; *)
-(*                                   msg_heap := qmsgs1; *)
-(*                                   c_heap := mycs1; *)
-(*                                   from_nons := froms1; *)
-(*                                   sent_nons := sents1; *)
-(*                                   cur_nonce := cur_n1 |}, iu, b0))). *)
-(*         ** eexists. *)
-(*            econstructor; eauto. *)
-(*            admit. *)
-(*            (* econstructor 2; eauto. *) *)
-(*            (* econstructor; eauto. *) *)
-(*            (* rewrite H24; trivial. *) *)
-
-(*            (* unfold syntactically_safe_U in *; split_ex; simpl in *. *) *)
-(*            (* generalize H0; intros USR; eapply H2 in USR; split_ex; eauto; simpl in *. *) *)
-
-(*            (* unfold goodness_predicates in *; simpl in *; *) *)
-(*            (*   split_ex; *) *)
-(*            (*   eapply action_matches_other_user_silent_step; eauto. *) *)
-
-(*         ** eexists. *)
-(*            econstructor; eauto. *)
-(*            (* econstructor 3; eauto. *) *)
-(*            (* econstructor; eauto. *) *)
-(*            (* rewrite H27; trivial. *) *)
-(*            admit. *)
-      
-(*       * exfalso. *)
-(*         dt x14; unfold build_data_step in H13; eapply labeled_action_never_commutes in H13; eauto; contradiction. *)
-
-(*       Unshelve. *)
-(*       all: eauto. *)
-(* Admitted. *)
-
-
-
 
 Lemma step_na :
   forall A B uid lbl bd
@@ -3315,10 +2788,6 @@ Proof.
   econstructor 2; eauto.
   econstructor 3; eauto.
   econstructor 4; eauto.
-
-  invert H8; [
-    econstructor 1
-  | econstructor 2]; simpl in *; eauto.
 Qed.
 
 Lemma violated_predicates_remain_violated :
@@ -3646,11 +3115,11 @@ Proof.
       invert H2.
       unfold build_data_step in *; rewrite <- H11 in H3; invert H3.
 
-    + invert H7; simpl in *.
+    + invert H6; simpl in *.
       eapply boundRunningTime_for_element in H2; eauto; split_ex.
       destruct x; try lia.
       invert H2.
-      unfold build_data_step in *; rewrite <- H9 in H3; invert H3.
+      unfold build_data_step in *; rewrite <- H11 in H3; invert H3.
 
   - destruct (classic (exists st', step st st')).
     + split_ex.
@@ -3709,7 +3178,7 @@ Qed.
 
 Hint Resolve many_steps_stays_lame many_steps_syntactically_safe many_steps_stays_good : core.
 
-Theorem step_stepC :
+Theorem step_stepC' :
   forall {t__hon t__adv} (ru0 : RealWorld.universe t__hon t__adv) (iu0 : IdealWorld.universe t__hon) b n summaries,
     runningTimeMeasure ru0 n
     -> goodness_predicates ru0
@@ -3757,6 +3226,227 @@ Proof.
     eapply violations_translate in H4; eauto; split_ex.
     apply INV in H4; eauto; split_ex.
     unfold not; intros; split_ex; contradiction.
+Qed.
+
+Lemma ss_implies_next_safe :
+  forall t (cmd : user_cmd t) uid ctx uids sty cs,
+    syntactically_safe uid uids ctx cmd sty
+    -> forall A B (usrs usrs' : honest_users A) (adv adv' : user_data B) cmd'
+        cs' gks gks' ks ks' qmsgs qmsgs' mycs mycs' froms froms' sents sents' n n' lbl,
+      step_user lbl (Some uid)
+                (usrs,adv,cs,gks,ks,qmsgs,mycs,froms,sents,n,cmd)
+                (usrs',adv',cs',gks',ks',qmsgs',mycs',froms',sents',n',cmd')
+      -> typingcontext_sound ctx usrs cs uid
+      -> uids = compute_ids usrs
+      -> forall t__n (cmd__n : user_cmd t__n), nextAction cmd cmd__n
+      -> (forall r, cmd__n <> Return r)
+      -> no_resends sents'
+      -> next_cmd_safe (findUserKeys usrs) cs uid froms sents cmd.
+Proof.
+  induct cmd;
+    unfold next_cmd_safe; intros;
+      match goal with
+      | [ H : nextAction _ _ |- _ ] => invert H
+      end; eauto;
+        try solve [ unfold typingcontext_sound in *; split_ex;
+                    match goal with
+                    | [ H : syntactically_safe _ _ _ _ _ |- _ ] => invert H
+                    end; eauto ].
+
+  - invert H0.
+    invert H1; eauto.
+    invert H4.
+    eapply IHcmd in H7; eauto.
+    eapply H7 in H11; eauto.
+
+    invert H11; trivial.
+
+  - unfold typingcontext_sound in *; split_ex; invert H.
+    apply H2 in H11; split_ex; subst.
+    apply H1 in H10.
+    unfold msg_honestly_signed, msg_signing_key,
+    msg_to_this_user, msg_destination_user,
+    msgCiphersSignedOk, honest_keyb;
+      context_map_rewrites.
+    destruct ( cipher_to_user x0 ==n cipher_to_user x0 ); try contradiction.
+    repeat simple apply conj; eauto.
+    econstructor; eauto.
+    unfold msg_honestly_signed, msg_signing_key, honest_keyb;
+      context_map_rewrites;
+      trivial.
+    (do 2 eexists); repeat simple apply conj; eauto.
+    invert H0.
+    unfold no_resends, updateSentNonce in H5; context_map_rewrites.
+    destruct (cipher_to_user x0 ==n cipher_to_user x0); try contradiction.
+    invert H5; eauto.
+    
+  - unfold typingcontext_sound in *; split_ex; invert H; eauto.
+    intros.
+    apply H12 in H; split_ex; subst; eauto.
+Qed.
+
+Lemma step_na_recur :
+  forall t t__n (cmd : user_cmd t) (cmd__n : user_cmd t__n),
+    nextAction cmd cmd__n
+    -> forall A B suid lbl bd bd',
+
+      step_user lbl suid bd bd'
+
+      -> forall cs cs' (usrs usrs': honest_users A) (adv adv' : user_data B) gks gks'
+          cmd__n' ks ks' qmsgs qmsgs' mycs mycs'
+          froms froms' sents sents' cur_n cur_n',
+
+        bd = (usrs, adv, cs, gks, ks, qmsgs, mycs, froms, sents, cur_n, cmd__n)
+        -> bd' = (usrs', adv', cs', gks', ks', qmsgs', mycs', froms', sents', cur_n', cmd__n')
+        -> exists bd'',
+            step_user lbl suid (usrs, adv, cs, gks, ks, qmsgs, mycs, froms, sents, cur_n, cmd) bd''.
+Proof.
+  induct 1; intros; subst;
+    eauto.
+
+  eapply IHnextAction in H0; eauto. split_ex.
+  simpl.
+
+  dt x; eexists; eapply StepBindRecur; eauto.
+Qed.
+
+Lemma ss_implies_next_safe_no_model_step :
+  forall A B (usrs : honest_users A) (adv : user_data B) cs gks
+    cmd uid ctx uids sty,
+
+    uids = compute_ids usrs
+    -> forall ks qmsgs mycs froms sents cur_n, usrs $? uid = Some (mkUserData ks cmd qmsgs mycs froms sents cur_n)
+    -> forall t__n (cmd__n : user_cmd t__n), nextAction cmd cmd__n
+    -> syntactically_safe uid uids ctx cmd sty
+    -> typingcontext_sound ctx usrs cs uid
+    -> forall ru iu, ru = mkUniverse usrs adv cs gks
+    -> (forall ru' iu', indexedModelStep uid (ru,iu,true) (ru',iu',true) -> False)
+    -> labels_align (ru,iu,true)
+    -> next_cmd_safe (findUserKeys usrs) cs uid froms sents cmd.
+Proof.
+  intros.
+  cases cmd__n;
+    unfold next_cmd_safe; intros;
+      match goal with
+      | [ H1 : nextAction cmd _, H2 : nextAction cmd _ |- _ ] => eapply na_deterministic in H1; eauto
+      end; split_ex; subst; trivial.
+
+  Ltac xyz :=
+    repeat 
+      match goal with
+      | [ NA : nextAction _ (Bind _ _) |- _ ] =>
+        eapply nextAction_couldBe in NA; contradiction
+      | [ SS : syntactically_safe _ _ _ ?cmd _, NA : nextAction ?cmd _ |- _ ] =>
+        eapply syntactically_safe_na in SS; eauto; split_ex
+      | [ SS : syntactically_safe _ _ _ _ _ |- _ ] =>
+        invert SS; unfold typingcontext_sound in *; split_ex; process_ctx
+      end.
+
+  all: xyz; eauto.
+
+  - exfalso.
+
+    assert (SEND : exists lbl bd,
+               step_user lbl
+                         (Some uid)
+                         (usrs, adv, cs, gks, ks, qmsgs, mycs, froms, sents, cur_n, 
+                          @Send t0 (cipher_to_user x0) (SignedCiphertext x)) bd).
+      (do 2 eexists); econstructor; clean_map_lookups; simpl in *; eauto.
+      context_map_rewrites; eauto.
+      unfold not; intros INV; invert INV; contradiction.
+      split_ex.
+
+      destruct x1.
+      invert H4.
+
+      dt x3.
+      eapply step_na_recur in H4; eauto; split_ex.
+      dt x1.
+
+      assert (exists ru', indexedRealStep uid (Action a)
+                                     (mkUniverse usrs adv cs gks)
+                                     ru')
+        by (eexists; econstructor; eauto). 
+      
+      split_ex.
+      generalize (H6 _ _ _ H8); intros; split_ex.
+      eapply H5; clear H5.
+      econstructor 2; eauto.
+
+  - eapply H11 in H4; split_ex.
+    eapply H in H4; eauto.
+Qed.
+
+Theorem step_stepC :
+  forall {t__hon t__adv} (ru0 : RealWorld.universe t__hon t__adv) (iu0 : IdealWorld.universe t__hon) b n summaries,
+    runningTimeMeasure ru0 n
+    -> goodness_predicates ru0
+    -> syntactically_safe_U ru0
+    -> summarize_univ ru0 summaries
+    -> lameAdv b ru0.(adversary)
+    -> invariantFor (TrS ru0 iu0) (fun st => no_resends_U (fst (fst st)) /\ alignment st)
+    -> invariantFor (TrS ru0 iu0) (fun st => safety st /\ alignment st)
+.
+Proof.
+  unfold invariantFor; intros.
+  specialize (H4 _ H5).
+  generalize H6; intros STEPS; eapply H4 in H6; eauto.
+  split_ex; split; eauto.
+
+  destruct s' as [[ru' iu'] b'].
+  simpl in *; split_ex; subst.
+  split_ors; try contradiction; subst.
+
+  assert (SS : syntactically_safe_U (fst (fst (ru', iu', true)))) by eauto.
+  unfold honest_cmds_safe; intros.
+
+  destruct (classic (exists st, indexedModelStep u_id (ru',iu',true) (st,true))).
+  - split_ex.
+    destruct x as [ru'' iu''].
+    pose proof (indexedModelStep_step H9) as STEP.
+    assert (STEPS' : (@step t__hon t__adv) ^* (ru',iu',true) (ru'',iu'',true)) by (eauto using TrcFront).
+    pose proof (trc_trans STEPS STEPS') as MORESTEPS.
+
+    specialize (H4 _ MORESTEPS); unfold no_resends_U in H4.
+    simpl in *; split_ex.
+
+    unfold syntactically_safe_U in SS;
+      specialize (SS _ _ _ H7 eq_refl); split_ex.
+
+    assert (exists lbl, indexedRealStep u_id lbl ru' ru'') by (invert H9; eauto).
+    split_ex.
+    invert H14.
+
+    unfold build_data_step, buildUniverse in *; simpl in *.
+    clean_map_lookups.
+
+    pose proof (na_always_exists (protocol userData)); split_ex.
+    destruct (classic (exists r, x3 = Return r)); split_ex; subst; eauto.
+    + unfold next_cmd_safe; intros.
+      eapply na_deterministic in H5; eauto.
+      split_ex; subst; trivial.
+
+    + rewrite Forall_natmap_forall in H4.
+      specialize (H4 u_id).
+      rewrite add_eq_o in H4 by trivial.
+      specialize (H4 _ eq_refl); simpl in H4.
+      eapply ss_implies_next_safe;
+        eauto.
+
+  - assert (forall st, indexedModelStep u_id (ru',iu',true) (st,true) -> False) by eauto using not_ex_all_not.
+    
+    subst.
+    clear H9.
+    unfold syntactically_safe_U in SS;
+      specialize (SS _ _ _ H7 eq_refl); split_ex.
+    simpl in *.
+
+    pose proof (na_always_exists (protocol u)); split_ex.
+    
+    destruct ru', u;
+      simpl in *;
+      eapply ss_implies_next_safe_no_model_step; eauto.
+
 Qed.
 
 Print Assumptions step_stepC.
